Interface entre forces_locale y M_basic

src/Renaming.thy
@@ -1,9 +1,9 @@
-theory Renaming imports Main Formula begin
+theory Renaming imports Formula begin
 
 section\<open>Renaming of free variables\<close>
 
 text\<open>TODO: this can be generalized to any pair of functions.\<close>
-
+(*
 definition 
   perm_n :: "[i,i] \<Rightarrow> i" where
   "perm_n(m,f) == \<lambda>n \<in> succ(m)  . if n=0 then 0 else succ(f`pred(n))"
@@ -80,12 +80,13 @@ definition perm_list :: "[i,i,i] \<Rightarrow> i" where
   "perm_list(f,l,i) ==  nat_rec(i,Nil,\<lambda> a e . e@[nth(f`a,l)])"
 
 (* TODO : nice property *)
+(*
 lemma perm_perm : "\<lbrakk> l \<in> list(A) ; f \<in> bij(length(l),length(l)) \<rbrakk> \<Longrightarrow>
    perm_list(converse(f),perm_list(f,l,length(l)),length(l)) = l"
   apply(induct_tac l,simp,unfold perm_list_def)
   apply(rule nat_rec_0)
-  oops
-    
+  sorry
+*)  
 consts   rename :: "i=>i"
 primrec
   "rename(Member(x,y)) =
@@ -146,12 +147,74 @@ lemma ren_tc [TC] : "p \<in> formula \<Longrightarrow>
   apply (simp,auto)
   apply(rule pred_le2,auto)
 done
+
+(*
+consts   rename :: "i=>i"
+primrec
+  "rename(Member(x,y)) =
+      (\<lambda> n \<in> nat . \<lambda>f \<in> bij(n,n). Member (f`x, f`y))"
+
+  "rename(Equal(x,y)) =
+      (\<lambda> n \<in> nat . \<lambda>f \<in> bij(n,n). Equal (f`x, f`y))"
+
+  "rename(Nand(p,q)) =
+      (\<lambda> n \<in> nat . \<lambda>f \<in> bij(n,n). Nand (rename(p)`n`f, rename(q)`n`f))"
+
+  "rename(Forall(p)) =
+      (\<lambda> n \<in> nat . \<lambda>f \<in> bij(n,n). Forall (rename(p) `succ(n)` perm_n(n,f)))"
+*)
+*)
+definition
+  swap_var :: "[i , i] \<Rightarrow> i" where
+  "swap_var(i,n) == if i=n then succ(i) else (if i=succ(n) then n else i)"
+
+lemma swap_var_type [TC] : 
+  "\<lbrakk> i \<in> nat ; n \<in> nat \<rbrakk> \<Longrightarrow> swap_var(i,n) \<in> nat"
+  by (simp add:swap_var_def)
+
+consts swap_suc :: "i\<Rightarrow>i" 
+primrec
+  "swap_suc(Member(x,y)) =
+    (\<lambda> n \<in> nat . Member(swap_var(x,n),swap_var(y,n)))"
+  "swap_suc(Equal(x,y)) = 
+    (\<lambda> n \<in> nat . Equal(swap_var(x,n),swap_var(y,n)))"
+  "swap_suc(Nand(p,q)) =
+    (\<lambda> n \<in> nat . Nand(swap_suc(p)`n,swap_suc(q)`n))"
+  "swap_suc(Forall(p)) =
+    (\<lambda> n \<in> nat . Forall(swap_suc(p)`(succ(n))))"
+
+lemma swap_suc_type [TC] : 
+  "\<lbrakk> \<phi> \<in> formula  \<rbrakk> \<Longrightarrow> swap_suc(\<phi>) \<in> nat \<rightarrow> formula"
+  by (induct_tac \<phi>,simp_all)
+
+lemma sats_swap_suc : 
+  "\<lbrakk> \<phi> \<in> formula ; n \<in> nat ; env \<in> list(M) ; env' \<in> list(M) ; n = length(env) \<rbrakk> \<Longrightarrow> 
+    sats(M,\<phi>,env@[a,b]@env') \<longleftrightarrow> sats(M,swap_suc(\<phi>)`n,env@[b,a]@env')"
+  sorry
+
+definition
+  swap_0_1 :: "i \<Rightarrow> i" where
+  "swap_0_1(\<phi>) == swap_suc(\<phi>)`0"
+
+lemma [TC] : "\<phi> \<in> formula \<Longrightarrow> swap_0_1(\<phi>) \<in> formula"
+  by (simp add: swap_0_1_def)
   
+
+lemma sats_swap_0_1 :
+  "\<lbrakk> \<phi> \<in> formula ; env \<in> list(M) ; a \<in> M ; b \<in> M\<rbrakk> \<Longrightarrow>
+  sats(M,swap_0_1(\<phi>),Cons(a,Cons(b,env))) \<longleftrightarrow> 
+  sats(M,\<phi>,Cons(b,Cons(a,env)))"
+  sorry
+
+(* sats(M, swap_0_1(\<phi>),Cons(xb, Cons(x, Cons(A, env)))*)
+
+(*
 lemma renSat : "p \<in> formula \<Longrightarrow> (\<forall> f . f \<in> bij(arity(p),arity(p)) \<longrightarrow> 
         arity(p) \<le> length(env) \<longrightarrow>  (* es necesario? *)
         sats(M,p,env) \<longrightarrow> 
         sats(M,rename(p)`f,perm_list(converse(f),env,length(env))))"
   apply (induct_tac p)
-  apply (unfold renActEnv_def)
-  apply (rule mem_iff_sats [THEN iffD1])  
-  apply (simp)
+     apply (simp)
+  sorry
+*)
+end
