forcing_posets.thy
@@ -181,8 +181,7 @@ lemma decr_seq_linear: "refl(P,leq) \<Longrightarrow> f \<in> nat -> P \<Longrig
     done
 
    
-lemma ball_distr_conj_iff: "(\<forall>x\<in>A. P(x) \<and> Q(x)) \<longleftrightarrow> (\<forall>x\<in>A. P(x)) \<and> (\<forall>x\<in>A. Q(x))"
- by blast
+lemmas ball_distr_conj_iff = upair.ball_conj_distrib 
     
 lemma subset_fun_image: "f:N\<rightarrow>P \<Longrightarrow> f``N\<subseteq>P"
   apply (simp add: image_fun)
