src/Forces_locale.thy
@@ -1,0 +1,22 @@
+theory Forces_locale imports Interface begin
+
+locale forcing_poset =
+  fixes P leq uno
+  assumes uno_in_P:         "uno \<in> P"
+      and leq_preord:       "preorder_on(P,leq)"
+      and uno_max:          "\<forall>p\<in>P. <p,uno>\<in>leq"
+
+locale forcing_data = forcing_poset +
+  fixes M enum
+  assumes trans_M:          "Transset(M)"
+      and M_model_ZF:       "satT(M,ZFTh,[])"
+      and M_countable:      "enum\<in>bij(nat,M)"
+      and P_in_M:           "P \<in> M"
+
+(* TODO: Quitar assumptions cuando tengamos el Relative hacked *)
+lemma (in forcing_data) to_M_basic :
+  "\<lbrakk> \<And>P. replacement(##M,P) ; nat \<in> M \<rbrakk> \<Longrightarrow> PROP M_basic(##M)"
+  by (insert trans_M M_model_ZF,rule interface_M_basic)
+
+
+end
